src/dafny/beacon/Helpers.s.dfy
@@ -12,15 +12,16 @@
  * under the License.
  */
 
+//  @dafny /dafnyVerify:1 /compile:0 /tracePOs /traceTimes /timeLimit:50 /noCheating:0
+
 include "../utils/Eth2Types.dfy"
 include "../utils/MathHelpers.dfy"
 include "../utils/NativeTypes.dfy"
+include "../utils/SetHelpers.dfy"
 include "../ssz/Constants.dfy"
 
 include "BeaconChainTypes.dfy"
 include "validators/Validators.dfy"
-
-
 
 /**
  *  Beacon chain helper functional specifications.
@@ -31,12 +32,29 @@ module BeaconHelperSpec {
     import opened Eth2Types
     import opened MathHelpers
     import opened NativeTypes
+    import opened SetHelpers
     import opened Constants
 
     import opened BeaconChainTypes
     import opened Validators
     import opened AttestationsTypes
     
+    // Predicates
+    /**
+     *  Check whether a set of validator indices are valid
+     *  i.e. within range such that index < |s.validators|.
+     *
+     *  @param      s       A beacon state.
+     *  @param      indices A sequence of validator indices as uint64.
+     *  @returns            True if all indices < |s.validators|.
+     */
+    predicate valid_state_indices(s: BeaconState, indices: seq<uint64>)
+    {
+        forall i :: 0 <= i < |indices| ==> indices[i] as int < |s.validators|
+    }
+
+
+    // Functions
 
     /**
      *  Collect pubkey in a list of validators.
@@ -53,15 +71,14 @@ module BeaconHelperSpec {
             { xv[0].pubkey } + keysInValidators(xv[1..])
     }
 
-
-
-    function get_VolExit_validator_indices(ve: seq<VoluntaryExit>): seq<int>
-        ensures |get_VolExit_validator_indices(ve)| == |ve|
-    {
-        if |ve| == 0 then []
-        else [ve[0].validator_index as int] + get_VolExit_validator_indices(ve[1..])
-    }
-
+    /**
+     *  Extract the list of validators from a sequence of proposer slashings.
+     *
+     *  @param      ps  A list of proposer slashings.
+     *  @returns        The sequence of validator indices for ps as ints.
+     *
+     *  @note           Return index type could be changed to uint64.
+     */
     function get_PS_validator_indices(ps: seq<ProposerSlashing>): seq<int>
         ensures |get_PS_validator_indices(ps)| == |ps|
     {
@@ -69,22 +86,132 @@ module BeaconHelperSpec {
         else [ps[0].header_1.proposer_index as int] + get_PS_validator_indices(ps[1..])
     }
 
+    /**
+     *  Extract the list of validators from a sequence of voluntary exits.
+     *
+     *  @param      ve  A list of voluntary exits.
+     *  @returns        The sequence of validator indices for ve as ints.
+     *
+     *  @note           Return index type could be changed to uint64 but int
+     *                  was used here for convenience.
+     */
+    function get_VolExit_validator_indices(ve: seq<VoluntaryExit>): seq<int>
+        ensures |get_VolExit_validator_indices(ve)| == |ve|
+    {
+        if |ve| == 0 then []
+        else [ve[0].validator_index as int] + get_VolExit_validator_indices(ve[1..])
+    }
 
+    /**
+     *  Sorted intersection of two sets of sorted validator indices.
+     *
+     *  @param      a   A sorted list of validators.
+     *  @param      b   A sorted list of validators.
+     *  @returns        The sorted intersection of a and b.
+     */
     function sorted_intersection_fn(a : seq<ValidatorIndex>, b: seq<ValidatorIndex>): seq<uint64>
         requires forall i,j :: 0 <= i < j < |a| ==> a[i] < a[j]
         requires forall i,j :: 0 <= i < j < |b| ==> b[i] < b[j]
-        ensures forall i,j :: 0 <= i < j < |sorted_intersection_fn(a,b)| ==> sorted_intersection_fn(a,b)[i] < sorted_intersection_fn(a,b)[j]
-        ensures forall i :: 0 <= i < |sorted_intersection_fn(a,b)| ==> sorted_intersection_fn(a,b)[i] as ValidatorIndex in a &&
-                                                                    sorted_intersection_fn(a,b)[i] as ValidatorIndex in b
+        ensures forall i,j :: 0 <= i < j < |sorted_intersection_fn(a,b)| 
+                ==> sorted_intersection_fn(a,b)[i] < sorted_intersection_fn(a,b)[j]
+        ensures forall i :: 0 <= i < |sorted_intersection_fn(a,b)| 
+                ==> sorted_intersection_fn(a,b)[i] as ValidatorIndex in a 
+                    && sorted_intersection_fn(a,b)[i] as ValidatorIndex in b
     {
         if |a| == 0 then []
         else (if a[0] in b then [a[0] as uint64] else []) + sorted_intersection_fn(a[1..], b)
     }
 
-    predicate valid_state_indices(s: BeaconState, indices: seq<uint64>)
+    /**
+     *  Get the total of a sequence of deposits as a nat.
+     *
+     *  @param      deposits    A sequence of deposits.
+     *  @returns                The total of all deposit amounts as a nat.
+     */
+    function total_deposits(deposits: seq<Deposit>): nat
     {
-        forall i :: 0 <= i < |indices| ==> indices[i] as int < |s.validators|
+        if |deposits| == 0 then 0
+        else total_deposits(deposits[..|deposits|-1]) + deposits[|deposits|-1].data.amount as nat
     }
-    
+
+    /**
+     *  Get the total of a sequence of balances as a nat.
+     *
+     *  @param      bal     A sequence of balance amounts.
+     *  @returns            The total of all balances as a nat.
+     */
+    function total_balances(bal: seq<Gwei>): nat
+    {
+        if |bal| == 0 then 0
+        else bal[0] as nat + total_balances(bal[1..])
+    }
+
+    /**
+     *  Collect set of indices of validators attesting a link.
+     *
+     *  @param  xa      A seq of attestations.
+     *  @param  src     The source checkpoint of the link.
+     *  @param  tgt     The target checkpoint of the link.
+     *  @returns        The set of validators's indices that vote for (src. tgt) in `xa`. 
+     */
+     function collectValidatorsAttestatingForLink(xa : seq<PendingAttestation>, src : CheckPoint, tgt: CheckPoint) : set<nat>
+        ensures forall e :: e in collectValidatorsAttestatingForLink(xa, src, tgt) ==>
+            e < MAX_VALIDATORS_PER_COMMITTEE as nat
+        ensures |collectValidatorsAttestatingForLink(xa, src, tgt)| <= MAX_VALIDATORS_PER_COMMITTEE as nat
+        decreases xa
+    {
+        if |xa| == 0 then 
+            { }
+        else 
+            unionCardBound(trueBitsCount(xa[0].aggregation_bits),
+                collectValidatorsAttestatingForLink(xa[1..], src, tgt), MAX_VALIDATORS_PER_COMMITTEE as nat);
+            (if xa[0].data.source == src && xa[0].data.target == tgt then 
+                trueBitsCount(xa[0].aggregation_bits)
+            else 
+                {}
+            ) + collectValidatorsAttestatingForLink(xa[1..], src, tgt)
+    }
+
+    /**
+     *  Collect set of indices of validators attesting a link to a given target.
+     *
+     *  @param  xa      A seq of attestations.
+     *  @param  tgt     The target checkpoint of the link.
+     *  @returns        The set of validators's indices that vote for (_. tgt) in `xa`. 
+     */
+    function collectValidatorsIndicesAttestatingForTarget(xa : seq<PendingAttestation>, tgt: CheckPoint) : set<nat>
+        ensures forall e :: e in collectValidatorsIndicesAttestatingForTarget(xa, tgt) ==>
+            e < MAX_VALIDATORS_PER_COMMITTEE as nat
+        ensures |collectValidatorsIndicesAttestatingForTarget(xa, tgt)| <= MAX_VALIDATORS_PER_COMMITTEE as nat
+        decreases xa
+    {
+        if |xa| == 0 then 
+            { }
+        else 
+            unionCardBound(trueBitsCount(xa[0].aggregation_bits),
+                collectValidatorsIndicesAttestatingForTarget(xa[1..], tgt), MAX_VALIDATORS_PER_COMMITTEE as nat);
+            (if xa[0].data.target == tgt then 
+                trueBitsCount(xa[0].aggregation_bits)
+            else 
+                {}
+            ) + collectValidatorsIndicesAttestatingForTarget(xa[1..], tgt)
+    }
+
+    /**
+     *  Collect the set of indices for which xb[i] is true.
+     *  
+     *  @param  xb  A sequence of bools.
+     *  @returns    The number of elements that are true in `xb`.
+     */
+    function trueBitsCount(xb : seq<bool>) : set<nat> 
+        ensures |trueBitsCount(xb)| <= |xb|
+        ensures forall i :: i in trueBitsCount(xb) <==> 0 <= i < |xb| && xb[i]
+        decreases xb
+    {
+        if |xb| == 0 then 
+            {}
+        else 
+            (if xb[|xb| - 1] then { |xb| - 1 } else {}) + trueBitsCount(xb[..|xb| - 1])
+    }
 
 }
